bv_exprs/bv-semantics.dfy
@@ -13,7 +13,7 @@ function bitwise_and(a:bv, b:bv) : (c:bv)
     ensures  |c| == |a|
 {
     if |a| == 0 then []
-    else [a[0] && b[0]] + bitwise_and(a[1..], b[1..])    
+    else [a[0] && b[0]] + bitwise_and(a[1..], b[1..])
 }
 
 function bitwise_or(a:bv, b:bv) : (c:bv)
@@ -21,12 +21,19 @@ function bitwise_or(a:bv, b:bv) : (c:bv)
     ensures  |c| == |a|
 {
     if |a| == 0 then []
-    else [a[0] || b[0]] + bitwise_or(a[1..], b[1..])    
+    else [a[0] || b[0]] + bitwise_or(a[1..], b[1..])
 }
 
-function xor(a:bool, b:bool) : bool
+function method xor(a:bool, b:bool) : bool
 {
     (a || b) && (!a || !b)
+}
+
+function bitwise_lsh(a:bv, b:nat) : (c:bv)
+	requires b <= |a|
+	ensures |c| == |a|
+{
+	seq(b, n => false) + a[0..(|a| - b)]
 }
 
 function bitwise_add_carry(a:bv, b:bv, c:bool) : (sum:bv)
@@ -34,7 +41,7 @@ function bitwise_add_carry(a:bv, b:bv, c:bool) : (sum:bv)
     ensures  |sum| == |a|
 {
     if |a| == 0 then []
-    else 
+    else
         var sum := xor(xor(a[0], b[0]), c);
         var c' := (a[0] && b[0]) || (c && (a[0] || b[0]));
         [sum] + bitwise_add_carry(a[1..], b[1..], c')
@@ -43,18 +50,54 @@ function bitwise_add_carry(a:bv, b:bv, c:bool) : (sum:bv)
 function bitwise_add(a:bv, b:bv) : bv
     requires |a| == |b|
 {
-    bitwise_add_carry(a, b, false) 
+    bitwise_add_carry(a, b, false)
+}
+
+function method bitwise_mul_partial(a:bv, b:bv, i:nat, j:nat) : (part:bool)
+	requires j <= i < |a| == |b|
+	decreases i - j
+{
+	if j == i then a[j] && b[0]
+	else
+		xor(a[j] && b[i-j], bitwise_mul_partial(a, b, i, j+1))
+}
+
+function method bitwise_mul(a:bv, b:bv) : (prod:bv)
+	requires |a| == |b|
+	ensures |prod| == |a|
+{
+	if |a| == 0 then []
+	else
+		seq(|a|, (n:nat) => if n < |a| then bitwise_mul_partial(a, b, n, 0) else false)
+}
+
+// test for bitwise_mul
+method Main()
+{
+	var a := [false, false]; // 0
+	var b := [true, true]; // 3
+	var c := [true, false]; // 1
+	var d := [false, true]; // 2
+
+  if bitwise_mul(a, b) == a { print "ok1\n"; }
+  if bitwise_mul(a, c) == a { print "ok2\n"; }
+  if bitwise_mul(a, d) == a { print "ok3\n"; }
+  if bitwise_mul(b, c) == b { print "ok4\n"; }
+  if bitwise_mul(b, d) == d { print "ok5\n"; } // (3 * 2) % 4 == 2
+  if bitwise_mul(c, d) == d { print "ok6\n"; }
 }
 
 datatype BinaryOp = And | Or | Add
+datatype ShiftOp = Lsh
 
 datatype BVExpr =
     | Const(bv)
     | Var(string)
     | Neg(e:BVExpr)
     | BinaryOp(op:BinaryOp, lhs:BVExpr, rhs:BVExpr)
-    
-datatype CmpOp = Eq | Neq //| Lt 
+		| ShiftOp(sh:ShiftOp, bve:BVExpr, amt:nat)
+
+datatype CmpOp = Eq | Neq //| Lt
 
 datatype CmpExpr = CmpExpr(op:CmpOp, lhs:BVExpr, rhs:BVExpr)
 
@@ -66,7 +109,7 @@ datatype LogicalExpr =
     | BinaryOp(op: LogicalBinaryOp, lhs:LogicalExpr, rhs:LogicalExpr)
 
 type store = map<string, bv>
-predicate ConsistentStore(s:store, w:nat) 
+predicate ConsistentStore(s:store, w:nat)
 {
     forall v :: v in s ==> |s[v]| == w
 }
@@ -79,19 +122,28 @@ function EvalBV(s:store, e:BVExpr, width:nat) : (r:Option<bv>)
     match e
         case Const(b) => if |b| >= width then Some(b[..width]) else None
         case Var(st) => if st in s then Some(s[st]) else None
-        case Neg(e) => 
+        case Neg(e) =>
             (match EvalBV(s, e, width)
             case None => None
             case Some(b) => Some(bitwise_neg(b)))
-        case BinaryOp(op, lhs, rhs) => 
+        case BinaryOp(op, lhs, rhs) =>
             var lhs := EvalBV(s, lhs, width);
             var rhs := EvalBV(s, rhs, width);
             if lhs.None? || rhs.None? then None
             else
-                match op
+                (match op
                 case And => Some(bitwise_and(lhs.v, rhs.v))
                 case Or  => Some(bitwise_or (lhs.v, rhs.v))
-                case Add => Some(bitwise_add(lhs.v, rhs.v))
+                case Add => Some(bitwise_add(lhs.v, rhs.v)))
+				case ShiftOp(sh, bve, amt) =>
+					var bve := EvalBV(s, bve, width);
+					if bve.None? then None
+					else
+						if amt > |bve.v| then None
+					else
+						match sh
+						case Lsh => Some(bitwise_lsh(bve.v, amt))
+
 }
 
 function EvalCmp(s:store, e:CmpExpr, width:nat) : Option<bool>
@@ -108,7 +160,7 @@ function EvalCmp(s:store, e:CmpExpr, width:nat) : Option<bool>
 
 predicate ValidCmpExprWidth(e:CmpExpr, w:nat)
 {
-    forall s :: 
+    forall s ::
         ConsistentStore(s, w) &&
         EvalCmp(s, e, w).Some?
         ==>
@@ -117,7 +169,7 @@ predicate ValidCmpExprWidth(e:CmpExpr, w:nat)
 
 predicate ValidCmpExpr(e:CmpExpr)
 {
-    forall s, width :: 
+    forall s, width ::
         ConsistentStore(s, width) &&
         EvalCmp(s, e, width).Some?
         ==>
@@ -128,8 +180,8 @@ function EvalLogicalExpr(s:store, e:LogicalExpr, width:nat) : Option<bool>
     requires ConsistentStore(s, width)
 {
     match e
-        case Cmp(e) => EvalCmp(s, e, width)        
-        case Not(e) => 
+        case Cmp(e) => EvalCmp(s, e, width)
+        case Not(e) =>
             (match EvalLogicalExpr(s, e, width)
                 case None => None
                 case Some(b) => Some(!b))
@@ -137,7 +189,7 @@ function EvalLogicalExpr(s:store, e:LogicalExpr, width:nat) : Option<bool>
             var lhs := EvalLogicalExpr(s, lhs, width);
             var rhs := EvalLogicalExpr(s, rhs, width);
             if lhs.None? || rhs.None? then None
-            else 
+            else
                 match op
                     case And => Some(lhs.v && rhs.v)
                     case Or  => Some(lhs.v || rhs.v)
@@ -145,10 +197,9 @@ function EvalLogicalExpr(s:store, e:LogicalExpr, width:nat) : Option<bool>
 
 predicate ValidLogicalExpr(e:LogicalExpr)
 {
-    forall s, width :: 
+    forall s, width ::
         ConsistentStore(s, width) &&
         EvalLogicalExpr(s, e, width).Some?
         ==>
         EvalLogicalExpr(s, e, width).v
 }
-
